new-semantics/coq/events/Syntax.v
@@ -1,12 +1,20 @@
 Inductive tm {var lbl} :=
-| tm_var (p : lbl) (x : var)
-| tm_lam (p : lbl)(x : var) (t : tm)
-| tm_app (p : lbl) (t1 t2 : tm)
-| tm_link (p : lbl) (t1 t2 : tm)
-| tm_mt (p : lbl)
-| tm_bind (p : lbl) (x : var) (t1 t2 : tm)
+| tm_var (x : var)
+| tm_lam (x : var) (t : ltm)
+| tm_app (t1 t2 : ltm)
+| tm_link (t1 t2 : ltm)
+| tm_mt
+| tm_bind (x : var) (t1 t2 : ltm)
+
+with ltm {var lbl} :=
+| lblled (p : lbl) (t : tm)
 .
 
+Scheme tm_ind_mut := Induction for tm Sort Prop
+  with ltm_ind_mut := Induction for ltm Sort Prop.
+
+Combined Scheme term_ind from tm_ind_mut, ltm_ind_mut.
+
 Variant val {var lbl} :=
-| v_fn (x : var) (t : @tm var lbl)
+| v_fn (x : var) (t : @ltm var lbl)
 .
